Assorted extra theorems and tools.  Added a new constant word_abs, which gives the absolute value of a bit-vector.

src/integer/integer_wordLib.sig
@@ -2,5 +2,8 @@ signature integer_wordLib =
 sig
     include Abbrev
 
+    val Cases_on_i2w     : term frag list -> tactic
+    val INT_SIZES_CONV   : conv
     val WORD_DECIDE      : conv (* Decision procedure, based on COOPER_PROVE *)
+
 end
